meeting hacking

compiler/backend/proofs/data_to_word_memoryProofScript.sml
@@ -697,89 +697,107 @@ Proof
   \\ res_tac \\ fs [ADDR_APPLY_def]
 QED
 
+(*
+TODO: remove?
 Theorem RTC_lemma[local]:
-  (*!r n. RTC (ref_edge refs) r n ==>
-          (!m. RTC (ref_edge refs) r m ==> bc_ref_inv conf m refs (f,tf,heap,be)) /\
-          gc_shared$gc_related g heap heap2 /\
-          f ' r IN FDOM g ==> f ' n IN FDOM g*)
   ∀r e.
     (ref_edge refs)꙳ r e ⇒
-      (e ∉ evaluated_thunk_ptr refs) ∧
       (∀m. (ref_edge refs)꙳ r m ⇒ bc_ref_inv conf m refs (f,tf,heap,be)) /\
       gc_shared$gc_related g heap heap2 ∧
-      f ' r ∈ FDOM g ⇒
-        f ' e ∈ FDOM g
+      f ' (SND r) ∈ FDOM g ⇒
+        f ' (SND e) ∈ FDOM g
 Proof
-  cheat
-  (*simp [RTC_eq_NRC, PULL_EXISTS]
-  \\ completeInduct_on `n` \\ gvs [] \\ rw []
-
-  \\ first_assum drule
-  \\ simp [bc_ref_inv_def]
-  \\ rpt (TOP_CASE_TAC \\ gvs []) \\ rw []
-  >- cheat
-  >- cheat
-  \\ gvs [ThunkBlock_def]
-  \\ Cases_on `n` \\ gvs [NRC]
-  \\ last_x_assum $ qspec_then `n'` assume_tac \\ gvs []
-  \\ pop_assum drule \\ reverse impl_tac >- gvs [] \\ rw []
-  >- cheat
-  >- (
-  )
-
-  \\ strip_tac \\ gvs []
-  \\ Cases_on `n` \\ gvs [NRC]
-  \\ gvs [bc_ref_inv_def, RefBlock_def, ThunkBlock_def]
-
   ho_match_mp_tac RTC_INDUCT \\ full_simp_tac std_ss [] \\ rpt strip_tac
-
   \\ full_simp_tac std_ss []
-  \\ first_x_assum irule \\ rw []
-  >- (first_x_assum irule \\ metis_tac [RTC_CASES1])
-  >- (first_x_assum irule \\ metis_tac [RTC_CASES1])
+  \\ qpat_x_assum `bb ==> bbb` match_mp_tac \\ full_simp_tac std_ss []
+  \\ strip_tac THEN1
+   (rpt strip_tac \\ qpat_x_assum `!x.bb` match_mp_tac \\ metis_tac [RTC_CASES1])
   \\ `RTC (ref_edge refs) r r' /\ RTC (ref_edge refs) r r` by metis_tac [RTC_CASES1]
-  \\ res_tac \\ rpt (qpat_x_assum `∀m. RTC _ _ _ ⇒ _` kall_tac)
+  \\ res_tac \\ qpat_x_assum `!x.bb` (K ALL_TAC)
+  \\ PairCases_on `r` \\ PairCases_on `r'`
   \\ full_simp_tac std_ss [bc_ref_inv_def,RefBlock_def,ThunkBlock_def,RTC_REFL]
-  \\ Cases_on `FLOOKUP f r` \\ full_simp_tac (srw_ss()) []
-  \\ Cases_on `FLOOKUP f r'` \\ full_simp_tac (srw_ss()) []
-  \\ Cases_on `lookup r refs` \\ full_simp_tac (srw_ss()) []
-  \\ Cases_on `lookup r' refs` \\ full_simp_tac (srw_ss()) []
+  \\ Cases_on `FLOOKUP f r1` \\ full_simp_tac (srw_ss()) []
+  \\ Cases_on `FLOOKUP f r'1` \\ full_simp_tac (srw_ss()) []
+  \\ Cases_on `lookup r1 refs` \\ full_simp_tac (srw_ss()) []
+  \\ Cases_on `lookup r'1 refs` \\ full_simp_tac (srw_ss()) []
   \\ Cases_on `x''` \\ full_simp_tac (srw_ss()) []
   \\ Cases_on `x'''` \\ full_simp_tac (srw_ss()) []
-
-  \\ gvs []
-  \\ drule_then assume_tac v_inv_related \\ gvs []
-  \\ gvs [ref_edge_def, get_refs_def, MEM_FLAT, MEM_MAP]
-  \\ gvs [gc_related_def, INJ_DEF, FLOOKUP_DEF]
-  \\ rpt (last_x_assum $ drule_at_then (Pat `_ ∈ FDOM g`) assume_tac)
-  \\ gvs [isSomeDataElement_def]
   >- (
-    drule_all_then assume_tac MEM_EVERY2_IMP \\ gvs []
-    \\ first_x_assum $ drule_at (Pat `v_inv _ _ _ _`) \\ gvs []
-    \\ impl_tac >- metis_tac [] \\ rw []
-    \\ gvs [EVERY_MEM, IN_DEF, evaluated_thunk_ptr_def])
+    drule_then assume_tac v_inv_related \\ gvs []
+    \\ gvs [gc_related_def]
+    \\ first_x_assum drule \\ gvs [FLOOKUP_DEF] \\ rw []
+    \\ gvs [ref_edge_def, get_refs_def, MEM_FLAT, MEM_MAP]
+    \\ drule_all MEM_EVERY2_IMP \\ rw []
+    \\ first_x_assum $ drule_at (Pos $ el 2) \\ gvs []
+    \\ impl_tac >- metis_tac [MEM_EL]
+    \\ rw []
+    \\ gvs [EVERY_MEM]
+    \\ first_x_assum drule \\ rw []
+    \\ gvs [IN_DEF, evaluated_thunk_ptr_def])
   >- (
-    drule_all_then assume_tac MEM_EVERY2_IMP \\ gvs []
-    \\ first_x_assum $ drule_at (Pat `v_inv _ _ _ _`) \\ gvs []
-    \\ impl_tac >- metis_tac [] \\ rw []
-    \\ gvs [EVERY_MEM, IN_DEF, evaluated_thunk_ptr_def])
+    drule_then assume_tac v_inv_related \\ gvs []
+    \\ gvs [gc_related_def]
+    \\ first_x_assum drule \\ gvs [FLOOKUP_DEF] \\ rw []
+    \\ gvs [ref_edge_def, get_refs_def, MEM_FLAT, MEM_MAP]
+    \\ drule_all MEM_EVERY2_IMP \\ rw []
+    \\ first_x_assum $ drule_at (Pos $ el 2) \\ gvs []
+    \\ impl_tac >- metis_tac [MEM_EL]
+    \\ rw []
+    \\ gvs [EVERY_MEM]
+    \\ first_x_assum drule \\ rw []
+    \\ gvs [IN_DEF, evaluated_thunk_ptr_def])
+   >- (
+    drule_then assume_tac v_inv_related \\ gvs []
+    \\ gvs [gc_related_def]
+    \\ first_x_assum drule \\ gvs [FLOOKUP_DEF] \\ rw []
+    \\ gvs [ref_edge_def, get_refs_def, MEM_FLAT, MEM_MAP]
+    \\ drule_all MEM_EVERY2_IMP \\ rw []
+    \\ first_x_assum $ drule_at (Pos $ el 2) \\ gvs []
+    \\ impl_tac >- metis_tac [MEM_EL]
+    \\ rw []
+    \\ gvs [EVERY_MEM]
+    \\ first_x_assum drule \\ rw []
+    \\ gvs [IN_DEF, evaluated_thunk_ptr_def]
+    \\ first_x_assum irule \\ gvs []
+    \\ CCONTR_TAC \\ gvs []
+    \\ cheat)
+  >- gvs [ref_edge_def]
+  >- gvs [ref_edge_def]
+  >- gvs [ref_edge_def]
   >- (
-    drule_all_then assume_tac MEM_EVERY2_IMP \\ gvs []
-    \\ first_x_assum $ drule_at (Pat `v_inv _ _ _ _`) \\ gvs []
-    \\ impl_tac >- metis_tac [] \\ rw []
-    \\ gvs [EVERY_MEM, IN_DEF, evaluated_thunk_ptr_def])
+    drule_then assume_tac v_inv_related \\ gvs []
+    \\ gvs [gc_related_def]
+    \\ first_x_assum drule \\ gvs [FLOOKUP_DEF] \\ rw []
+    \\ gvs [ref_edge_def, get_refs_def, MEM_FLAT, MEM_MAP]
+    \\ first_x_assum $ drule_at (Pos $ el 2) \\ gvs []
+    \\ rw []
+    \\ gvs [EVERY_MEM]
+    \\ first_x_assum drule \\ rw []
+    \\ gvs [IN_DEF, evaluated_thunk_ptr_def])
   >- (
-    first_x_assum $ drule_at (Pat `v_inv _ _ _ _`) \\ gvs []
-    \\ gvs [EVERY_MEM, IN_DEF, evaluated_thunk_ptr_def])
+    drule_then assume_tac v_inv_related \\ gvs []
+    \\ gvs [gc_related_def]
+    \\ first_x_assum drule \\ gvs [FLOOKUP_DEF] \\ rw []
+    \\ gvs [ref_edge_def, get_refs_def, MEM_FLAT, MEM_MAP]
+    \\ first_x_assum $ drule_at (Pos $ el 2) \\ gvs []
+    \\ rw []
+    \\ gvs [EVERY_MEM]
+    \\ first_x_assum drule \\ rw []
+    \\ gvs [IN_DEF, evaluated_thunk_ptr_def])
   >- (
-    first_x_assum $ drule_at (Pat `v_inv _ _ _ _`) \\ gvs []
-    \\ gvs [EVERY_MEM, IN_DEF, evaluated_thunk_ptr_def])
-  >- (
-    qpat_x_assum `v_inv _ _ _ (z',_,_,_)` kall_tac
-    \\ first_x_assum $ drule_at (Pat `v_inv _ _ _ _`) \\ gvs []
-    \\ gvs [EVERY_MEM, IN_DEF])
-
-  *)
+    drule_then assume_tac v_inv_related \\ gvs []
+    \\ gvs [gc_related_def]
+    \\ first_x_assum drule \\ gvs [FLOOKUP_DEF] \\ rw []
+    \\ gvs [ref_edge_def, get_refs_def, MEM_FLAT, MEM_MAP]
+    \\ qpat_x_assum `v_inv _ _ _ _` mp_tac
+    \\ first_x_assum $ drule_at (Pos $ el 2) \\ gvs []
+    \\ rw []
+    \\ gvs [EVERY_MEM]
+    \\ first_x_assum drule \\ rw []
+    \\ gvs [IN_DEF, evaluated_thunk_ptr_def]
+    \\ first_x_assum irule \\ gvs []
+    \\ CCONTR_TAC \\ gvs []
+    \\ cheat)
 QED
 
 Theorem reachable_refs_lemma[local]:
@@ -808,30 +826,9 @@ Proof
   \\ `(!m. RTC (ref_edge refs) r m ==>
            bc_ref_inv conf m refs (f,tf,heap,be))` by metis_tac []
   \\ drule RTC_lemma
-  \\ disch_then drule
-
-
-  NTAC 3 strip_tac \\ full_simp_tac std_ss [reachable_refs_def,PULL_EXISTS]
-  \\ `?xs1 xs2. stack = xs1 ++ x::xs2` by metis_tac [MEM_SPLIT]
-  \\ full_simp_tac std_ss [] \\ imp_res_tac LIST_REL_SPLIT1
-  \\ full_simp_tac std_ss [LIST_REL_CONS1] \\ rveq
-  \\ full_simp_tac std_ss [MEM,MEM_APPEND,LIST_REL_CONS1]
-  \\ full_simp_tac std_ss [EVERY_MEM] \\ res_tac \\ full_simp_tac std_ss []
-  \\ `EVERY (\n. n ∉ evaluated_thunk_ptr refs ⇒ f ' n IN FDOM g) (get_refs x)`
-    by metis_tac [v_inv_related]
-  \\ `n IN FDOM f` by (CCONTR_TAC
-    \\ full_simp_tac (srw_ss()) [bc_ref_inv_def,FLOOKUP_DEF])
-  \\ full_simp_tac std_ss []
-  \\ `bc_ref_inv conf r refs (f,tf,heap,be)` by metis_tac [RTC_REFL]
-  \\ `(!m. RTC (ref_edge refs) r m ==>
-           bc_ref_inv conf m refs (f,tf,heap,be))` by metis_tac []
-  \\ `r ∉ evaluated_thunk_ptr refs` by metis_tac [RTC_REFL]
-  \\ `(∀m. (ref_edge refs)꙳ r m ⇒
-            m ∉ evaluated_thunk_ptr refs)` by metis_tac []
-  \\ irule RTC_lemma
-  \\ rpt (goal_assum (drule_at Any) \\ gvs [])
-  \\ gvs [EVERY_MEM]*)
+  \\ disch_then drule*)
 QED
+*)
 
 Inductive gc_inline_rel:
 [~unchanged:] gc_inline_rel inline h1 x x
@@ -1014,23 +1011,57 @@ Proof
   >- (
     drule gc_heap_inline_rel_v_inv \\ gvs []
     \\ gvs [LIST_REL_EL_EQN] \\ rw []
-    \\ metis_tac [])
-  \\ gvs [bc_ref_inv_def, FLOOKUP_DEF]
-  \\ first_x_assum drule_all \\ gvs [] \\ strip_tac \\ gvs []
+    \\ first_x_assum irule \\ gvs [] \\ rw []
+    >- (
+      qexists `be` \\ rw [] \\ gvs []
+      \\ first_x_assum irule \\ gvs [reachable_refs_def, MEM_EL]
+      \\ simp [PULL_EXISTS]
+      \\ ntac 2 (first_x_assum $ irule_at $ Pos hd \\ gvs []))
+    \\ first_x_assum $ irule_at $ Pos hd \\ gvs [])
+  \\ first_assum drule \\ impl_tac >- simp []
+  \\ pure_rewrite_tac [bc_ref_inv_def] \\ rw []
+  \\ gvs [FLOOKUP_DEF]
   \\ ntac 2 (TOP_CASE_TAC \\ gvs [])
-  >- cheat
-  >- cheat
   >- (
-    drule gc_heap_inline_rel_v_inv
-    \\ disch_then drule
-    \\ gvs [LIST_REL_EL_EQN]
-    \\ qpat_x_assum `∀n. n < LENGTH heap2 ⇒ gc_heap_inline_rel _ _ _ _` mp_tac
-    \\ disch_then $ qspec_then `f ' n` mp_tac \\ gvs []
-    \\ impl_tac >- cheat
-    \\ simp [gc_heap_inline_rel_cases]
+    drule LIST_REL_gc_heap_inline_DataElement \\ gvs [RefBlock_def]
+    \\ disch_then drule \\ rw [] \\ simp []
+    \\ pop_assum mp_tac
+    \\ rw [LIST_REL_EL_EQN] >- gvs [LIST_REL_EL_EQN]
+    \\ irule gc_heap_inline_rel_v_inv \\ gvs []
+    \\ first_x_assum $ irule_at (Pos $ el 2)
+    \\ first_x_assum $ drule_then assume_tac \\ gvs []
+    \\ pop_assum $ irule_at Any \\ gvs []
+    \\ qexists `be` \\ conj_tac \\ gvs []
+    >- (
+      rw []
+      \\ first_x_assum irule \\ gvs [reachable_refs_def]
+      \\ ntac 2 (first_x_assum $ irule_at (Pos hd) \\ gvs [])
+      \\ irule RTC_TRANS
+      \\ first_x_assum $ irule_at (Pos hd) \\ gvs []
+      \\ simp [Once RTC_CASES1]
+      \\ disj2_tac \\ gvs [ref_edge_def, get_refs_def, MEM_FLAT, MEM_MAP]
+      \\ pop_assum $ irule_at Any \\ gvs []
+      \\ first_x_assum $ irule_at Any \\ gvs [MEM_EL, LIST_REL_EL_EQN]
+      \\ irule_at Any EQ_REFL \\ gvs [])
+    \\ gvs [LIST_REL_EL_EQN])
+  >- (
+    drule LIST_REL_gc_heap_inline_DataElement \\ gvs [Bytes_def]
+    \\ disch_then drule \\ rw [] \\ simp [])
+  >- (
+    drule LIST_REL_gc_heap_inline_DataElement \\ gvs [ThunkBlock_def]
+    \\ disch_then drule \\ rw [] \\ simp []
+    \\ irule gc_heap_inline_rel_v_inv \\ gvs []
+    \\ ntac 2 (first_x_assum $ irule_at (Pos $ el 2))
+    \\ simp []
+    \\ qexists `be` \\ gvs []
     \\ rw []
-    >- cheat
-  )
+    \\ first_x_assum irule \\ gvs [reachable_refs_def]
+    \\ ntac 2 (first_x_assum $ irule_at (Pos hd) \\ gvs [])
+    \\ irule RTC_TRANS
+    \\ first_x_assum $ irule_at (Pos hd) \\ gvs []
+    \\ simp [Once RTC_CASES1]
+    \\ disj2_tac \\ gvs [ref_edge_def, get_refs_def, MEM_FLAT, MEM_MAP]
+    \\ pop_assum $ irule_at Any \\ gvs [])
 QED
 
 Theorem bc_stack_ref_inv_gc_related_roots_heap[local]:
@@ -1060,7 +1091,7 @@ Proof
 QED
 
 Theorem bc_stack_ref_inv_related[local]:
-  gc_inline_related dest_evaluated_thunk g (roots1,heap1) (roots2,heap2) ∧
+  gc_inline_related dest_evaluated_thunk_rel g (roots1,heap1) (roots2,heap2) ∧
   bc_stack_ref_inv conf ts stack refs (roots1,heap1,be) ⇒
     bc_stack_ref_inv conf ts stack refs (roots2,heap2,be)
 Proof
@@ -1169,8 +1200,7 @@ Theorem full_gc_thm:
       all_reachable_from_roots roots2 (heap2 ++ heap_expand (limit - a2)) /\
       EVERY isDataElement heap2
 Proof
-  cheat
-  (*simp_tac std_ss [abs_ml_inv_def,GSYM CONJ_ASSOC]
+  simp_tac std_ss [abs_ml_inv_def,GSYM CONJ_ASSOC]
   \\ rpt strip_tac \\ old_drule full_gc_related
   \\ asm_simp_tac std_ss [] \\ strip_tac
   \\ qpat_x_assum `heap_length heap2 = _` (assume_tac o GSYM)
@@ -1189,7 +1219,12 @@ Proof
   \\ reverse conj_tac THEN1 metis_tac []
   \\ reverse conj_tac THEN1
    (match_mp_tac (GEN_ALL bc_stack_ref_inv_related) \\ full_simp_tac std_ss []
-    \\ qexists_tac `heap` \\ full_simp_tac std_ss []
+    \\ simp [gc_inline_related_def, PULL_EXISTS, gc_inline_def]
+    \\ qexistsl [`roots`, `heap`, `f`, `roots`, `heap`] \\ simp []
+    \\ simp [GSYM CONJ_ASSOC]
+    \\ conj_tac >- (irule EVERY2_refl \\ simp [gc_inline_rel_cases])
+    \\ conj_tac >- (irule EVERY2_refl \\ simp [gc_heap_inline_rel_cases])
+    \\ simp [gc_related_roots_heap_def]
     \\ rw [] \\ fs [] \\ res_tac \\ fs []
     \\ fs [reachable_addresses_def,IN_DEF]
     \\ asm_exists_tac \\ fs [])
@@ -1197,7 +1232,7 @@ Proof
    (qpat_x_assum `full_gc (roots,heap,limit) = xxx` (ASSUME_TAC o GSYM)
     \\ imp_res_tac full_gc_ok \\ NTAC 3 (POP_ASSUM (K ALL_TAC))
     \\ full_simp_tac std_ss [] \\ metis_tac [])
-  \\ fs [gc_kind_inv_def] \\ CASE_TAC \\ fs []*)
+  \\ fs [gc_kind_inv_def] \\ CASE_TAC \\ fs []
 QED
 
 Definition make_gc_conf_def:
@@ -1367,8 +1402,7 @@ Theorem gen_gc_thm:
       all_reachable_from_roots roots2
         (state2.h1 ++ heap_expand state2.n ++ state2.r1)
 Proof
-  cheat
-  (*simp_tac std_ss [abs_ml_inv_def,GSYM CONJ_ASSOC,make_gc_conf_def]
+  simp_tac std_ss [abs_ml_inv_def,GSYM CONJ_ASSOC,make_gc_conf_def]
   \\ rpt strip_tac \\ qmatch_goalsub_abbrev_tac `gen_gc cc`
   \\ `heap_ok heap cc.limit` by fs [Abbr `cc`]
   \\ old_drule gen_gcTheory.gen_gc_related
@@ -1380,7 +1414,12 @@ Proof
   THEN1 (match_mp_tac IMP_all_reachable_from_roots \\ fs [])
   THEN1
    (match_mp_tac (GEN_ALL bc_stack_ref_inv_related) \\ full_simp_tac std_ss []
-    \\ qexists_tac `heap` \\ full_simp_tac std_ss []
+    \\ simp [gc_inline_related_def, PULL_EXISTS, gc_inline_def]
+    \\ qexistsl [`roots`, `heap`, `f`, `roots`, `heap`] \\ simp []
+    \\ simp [GSYM CONJ_ASSOC]
+    \\ conj_tac >- (irule EVERY2_refl \\ simp [gc_inline_rel_cases])
+    \\ conj_tac >- (irule EVERY2_refl \\ simp [gc_heap_inline_rel_cases])
+    \\ simp [gc_related_roots_heap_def]
     \\ rw [] \\ fs [] \\ res_tac \\ fs []
     \\ fs [reachable_addresses_def,IN_DEF] \\ asm_exists_tac \\ fs [])
   THEN1
@@ -1404,7 +1443,7 @@ Proof
     \\ once_rewrite_tac [ADD_COMM]
     \\ pop_assum (fn thm => PURE_ONCE_REWRITE_TAC [thm])
     \\ PURE_ONCE_REWRITE_TAC [gen_gc_partialTheory.heap_split_length]
-    \\ fs[heap_expand_not_isRef])*)
+    \\ fs[heap_expand_not_isRef])
 QED
 
 Definition has_gen_def:
@@ -1463,8 +1502,7 @@ Theorem gen_gc_partial_thm:
         (roots2,state2.old ++ state2.h1 ++ heap_expand state2.n ++ state2.r1,be,
          state2.a,state2.n,0,reset_gens conf state2.a) limit ts /\ state2.ok
 Proof
-  cheat
-  (*simp_tac std_ss [abs_ml_inv_def,GSYM CONJ_ASSOC,make_gc_conf_def]
+  simp_tac std_ss [abs_ml_inv_def,GSYM CONJ_ASSOC,make_gc_conf_def]
   \\ rpt strip_tac \\ qmatch_goalsub_abbrev_tac `partial_gc cc`
   \\ `heap_ok heap cc.limit` by
         (fs [Abbr `cc`] \\ Cases_on `gens` \\ fs [make_partial_conf_def])
@@ -1511,7 +1549,12 @@ Proof
   \\ fs []
   \\ reverse (rpt conj_tac) THEN1
    (match_mp_tac (GEN_ALL bc_stack_ref_inv_related) \\ full_simp_tac std_ss []
-    \\ qexists_tac `heap` \\ full_simp_tac std_ss []
+    \\ simp [gc_inline_related_def, PULL_EXISTS, gc_inline_def]
+    \\ qexistsl [`roots`, `heap`, `f`, `roots`, `heap`] \\ simp []
+    \\ simp [GSYM CONJ_ASSOC]
+    \\ conj_tac >- (irule EVERY2_refl \\ simp [gc_inline_rel_cases])
+    \\ conj_tac >- (irule EVERY2_refl \\ simp [gc_heap_inline_rel_cases])
+    \\ simp [gc_related_roots_heap_def]
     \\ rw [] \\ fs [] \\ res_tac \\ fs [])
   THEN1
    (qpat_abbrev_tac `hh = state'.old ++ state'.h1`
@@ -1586,7 +1629,7 @@ Proof
   \\ res_tac
   \\ qmatch_goalsub_abbrev_tac `heap_lookup _ heap2`
   \\ fs [gc_related_def,isSomeDataElement_def]
-  \\ res_tac \\ fs []*)
+  \\ res_tac \\ fs []
 QED
 
 Definition data_pointers_def:
@@ -2039,6 +2082,11 @@ Proof
     \\ drule_all heap_store_rel_lemma \\ gvs [])
   >- (gvs [SUBMAP_DEF] \\ rpt (TOP_CASE_TAC \\ gvs []))
   >- (
+    disj1_tac \\ gvs []
+    \\ gvs [FLOOKUP_DEF, SUBMAP_DEF, heap_store_rel_def, ThunkBlock_def]
+    \\ first_x_assum $ qspec_then ‘f1 ' n’ assume_tac
+    \\ gvs [isSomeDataElement_def])
+  >- (
     irule_at Any EQ_REFL \\ gvs [BlockRep_def]
     \\ gvs [FLOOKUP_DEF, SUBMAP_DEF, heap_store_rel_def, BlockRep_def]
     \\ first_x_assum $ qspec_then ‘tf1 ' ts’ assume_tac
@@ -2318,21 +2366,52 @@ Theorem v_inv_lemma:
                              ha++hs++heap_expand (sp - heap_length hs)++hb)
 Proof
   ho_match_mp_tac v_inv_rel_strongind \\ rw [] \\ gvs [v_inv_def]
-  \\ rpt (TOP_CASE_TAC \\ gvs [])
-  \\ unlength_tac [heap_lookup_APPEND, heap_length_APPEND, heap_expand_def]
-  \\ fs [case_eq_thms]
-  \\ namedCases_on `sp` ["", "sp'"] \\ fs []
-  \\ fs [heap_lookup_def, Bignum_def, Word64Rep_def, BlockRep_def]
-  \\ rpt (pairarg_tac \\ fs [])
-  \\ unlength_tac [ADD1]
-  \\ IF_CASES_TAC \\ fs []
-  \\ TRY (qexists_tac `xs`)
-  \\ fs [LIST_REL_EL_EQN] \\ rw []
-  \\ unlength_tac []
-  \\ rpt (AP_THM_TAC ORELSE AP_TERM_TAC) \\ fs []
-  \\ imp_res_tac heap_lookup_SPLIT
-  \\ gvs[]
-  \\ unlength_tac [heap_lookup_APPEND, heap_length_APPEND, heap_lookup_def]
+  >- (
+    unlength_tac [heap_lookup_APPEND, heap_length_APPEND, heap_expand_def]
+    \\ fs [case_eq_thms]
+    \\ namedCases_on `sp` ["", "sp'"] \\ fs []
+    \\ fs [heap_lookup_def, Bignum_def, Word64Rep_def, BlockRep_def]
+    \\ rpt (pairarg_tac \\ fs [])
+    \\ unlength_tac [ADD1]
+    \\ IF_CASES_TAC \\ fs []
+    \\ imp_res_tac heap_lookup_SPLIT \\ gvs[]
+    \\ unlength_tac [heap_lookup_APPEND, heap_length_APPEND, heap_lookup_def])
+  >- (
+    unlength_tac [heap_lookup_APPEND, heap_length_APPEND, heap_expand_def]
+    \\ fs [case_eq_thms]
+    \\ namedCases_on `sp` ["", "sp'"] \\ fs []
+    \\ fs [heap_lookup_def, Bignum_def, Word64Rep_def, BlockRep_def]
+    \\ rpt (IF_CASES_TAC \\ gvs [])
+    \\ imp_res_tac heap_lookup_SPLIT \\ gvs[]
+    \\ unlength_tac [heap_lookup_APPEND, heap_length_APPEND, heap_lookup_def])
+  >- (
+    disj1_tac \\ gvs []
+    \\ unlength_tac [heap_lookup_APPEND, heap_length_APPEND, heap_expand_def]
+    \\ fs [case_eq_thms]
+    >- (irule_at (Pos hd) EQ_REFL \\ gvs [])
+    \\ namedCases_on `sp` ["", "sp'"] \\ gvs [ThunkBlock_def]
+    \\ fs [heap_lookup_def, Bignum_def, Word64Rep_def, BlockRep_def]
+    \\ unlength_tac [ADD1]
+    \\ IF_CASES_TAC \\ gvs []
+    \\ imp_res_tac heap_lookup_SPLIT \\ gvs[]
+    \\ unlength_tac [heap_lookup_APPEND, heap_length_APPEND, heap_lookup_def]
+    \\ once_rewrite_tac [GSYM APPEND_ASSOC]
+    \\ once_rewrite_tac [GSYM CONS_APPEND]
+    \\ simp [])
+  >- (
+    unlength_tac [heap_lookup_APPEND, heap_length_APPEND, heap_expand_def]
+    \\ fs [case_eq_thms]
+    >- (
+      namedCases_on `sp` ["", "sp'"] \\ fs []
+      \\ fs [heap_lookup_def, Bignum_def, Word64Rep_def, BlockRep_def]
+      \\ rpt (IF_CASES_TAC \\ gvs [])
+      \\ gvs [LIST_REL_EL_EQN])
+    \\ namedCases_on `sp` ["", "sp'"] \\ fs []
+    \\ fs [heap_lookup_def, Bignum_def, Word64Rep_def, BlockRep_def]
+    \\ rpt (IF_CASES_TAC \\ gvs [])
+    \\ qexists `xs` \\ gvs [LIST_REL_EL_EQN]
+    \\ imp_res_tac heap_lookup_SPLIT \\ gvs[]
+    \\ unlength_tac [heap_lookup_APPEND, heap_length_APPEND, heap_lookup_def])
 QED
 
 Theorem v_inv_lemma[allow_rebind]:
@@ -2761,7 +2840,9 @@ Theorem v_inv_tf_update_thm_lemma:
           v_inv conf v refs (y,f, tf |+ (ts',a),heap)
 Proof
   ho_match_mp_tac v_inv_rel_strongind \\ rw [] \\ gvs [v_inv_def]
-  \\ rpt (TOP_CASE_TAC \\ gvs [])
+  >- (
+    disj1_tac \\ gvs []
+    \\ irule_at Any EQ_REFL \\ gvs [FLOOKUP_UPDATE, FLOOKUP_DEF])
   \\ irule_at Any EQ_REFL \\ gvs [FLOOKUP_UPDATE, FLOOKUP_DEF]
   \\ IF_CASES_TAC \\ gvs [LIST_REL_EL_EQN] \\ rw []
 QED
@@ -2784,11 +2865,15 @@ Theorem v_inv_tf_update_thm_alt_lemma:
           v_inv conf v refs (y,f, tf |+ (ts', a),heap)
 Proof
   ho_match_mp_tac v_inv_rel_strongind \\ rw []
-  \\ gvs [v_inv_def, BlockRep_def, v_all_ts_def]
+  \\ gvs [v_inv_def, BlockRep_def, ThunkBlock_def, v_all_ts_def]
   >- (
     disj1_tac \\ gvs []
-    \\ first_x_assum irule \\ gvs []
-    \\ gvs [all_ts_def]
+    \\ first_x_assum irule \\ gvs [all_ts_def]
+    \\ first_x_assum $ qspec_then ‘v’ assume_tac \\ gvs []
+    \\ first_x_assum $ qspec_then ‘n’ assume_tac \\ gvs [])
+  >- (
+    disj2_tac \\ gvs []
+    \\ first_x_assum irule \\ gvs [all_ts_def]
     \\ first_x_assum $ qspec_then ‘v’ assume_tac \\ gvs []
     \\ first_x_assum $ qspec_then ‘n’ assume_tac \\ gvs [])
   >- (
@@ -2841,6 +2926,16 @@ Proof
       \\ metis_tac [MEM_in_all_vs])
     >- (
       disj1_tac \\ gvs []
+      \\ irule_at (Pos hd) EQ_REFL \\ gvs []
+      \\ irule v_inv_tf_update_thm_alt \\ gvs []
+      \\ first_assum $ irule_at Any \\ gvs []
+      \\ CCONTR_TAC \\ gvs []
+      \\ drule_at_then Any assume_tac MEM_in_all_ts \\ gvs []
+      \\ pop_assum $ qspecl_then [‘stack’, ‘refs’] assume_tac \\ gvs []
+      \\ gvs [all_vs_def]
+      \\ first_x_assum $ qspec_then ‘n'’ assume_tac \\ gvs [MEM_v_all_vs])
+    >- (
+      disj2_tac \\ gvs []
       \\ irule v_inv_tf_update_thm_alt \\ gvs []
       \\ first_assum $ irule_at Any \\ gvs []
       \\ CCONTR_TAC \\ gvs []
@@ -2875,6 +2970,14 @@ Proof
   ho_match_mp_tac v_inv_rel_strongind \\ rw [] \\ gvs [v_inv_def]
   >- (
     disj1_tac \\ gvs [v_all_ts_def]
+    \\ irule_at (Pos hd) EQ_REFL \\ gvs []
+    \\ ntac 2 (first_x_assum irule \\ rw [])
+    \\ gvs [all_ts_def]
+    \\ first_assum $ irule_at Any \\ gvs []
+    \\ disj1_tac \\ gvs []
+    \\ first_x_assum $ irule_at Any \\ gvs [])
+  >- (
+    disj2_tac \\ gvs [v_all_ts_def]
     \\ ntac 2 (first_x_assum irule \\ rw [])
     \\ gvs [all_ts_def]
     \\ first_assum $ irule_at Any \\ gvs []
@@ -3005,7 +3108,7 @@ Proof
     \\ match_mp_tac (GEN_ALL v_inv_SUBMAP)
     \\ goal_assum (first_x_assum o mp_then Any mp_tac)
     \\ fs [])
-  \\ `reachable_refs (xs++stack) refs n` by
+  \\ `reachable_refs (xs++stack) refs (b,n)` by
    (ntac 2 $ POP_ASSUM MP_TAC \\ simp_tac std_ss [reachable_refs_def]
     \\ rpt strip_tac \\ full_simp_tac std_ss [MEM] THEN1
      (NTAC 2 (POP_ASSUM MP_TAC) \\ full_simp_tac std_ss []
@@ -3057,7 +3160,7 @@ Proof
   \\ qexists_tac `tf` \\ full_simp_tac std_ss []
   \\ fs [all_ts_cons,SUBSET_INSERT_RIGHT]
   \\ full_simp_tac (srw_ss()) [v_inv_def]
-  \\ rpt strip_tac \\ sg `reachable_refs stack refs n` \\ res_tac
+  \\ rpt strip_tac \\ sg `reachable_refs stack refs (b,n)` \\ res_tac
   \\ full_simp_tac std_ss [reachable_refs_def]
   \\ Cases_on `x = Block 0 tag []` \\ full_simp_tac std_ss []
   \\ full_simp_tac (srw_ss()) [get_refs_def] \\ metis_tac []
@@ -3346,8 +3449,9 @@ QED
 (* update ref *)
 
 Theorem ref_edge_ValueArray[local]:
-  ref_edge (insert ptr (ValueArray xs) refs) x y =
-    if x = ptr then MEM y (get_refs (Block 0 ARB xs)) else ref_edge refs x y
+  ref_edge (insert ptr (ValueArray xs) refs) (bx,x) (by,y) =
+    if x = ptr then MEM (by,y) (get_refs (Block 0 ARB xs))
+               else ref_edge refs (bx,x) (by,y)
 Proof
   simp_tac std_ss [FUN_EQ_THM,ref_edge_def] \\ rpt strip_tac
   \\ full_simp_tac (srw_ss()) [FLOOKUP_DEF,FAPPLY_FUPDATE_THM]
@@ -3356,8 +3460,9 @@ Proof
 QED
 
 Theorem ref_edge_Thunk[local]:
-  ref_edge (insert ptr (Thunk ev v) refs) x y =
-    if x = ptr then MEM y (get_refs (Block 0 ARB [v])) else ref_edge refs x y
+  ref_edge (insert ptr (Thunk ev v) refs) (bx,x) (by,y) =
+    if x = ptr then MEM (by,y) (get_refs (Block 0 ARB [v]))
+               else ref_edge refs (bx,x) (by,y)
 Proof
   simp_tac std_ss [FUN_EQ_THM,ref_edge_def] \\ rpt strip_tac
   \\ full_simp_tac (srw_ss()) [FLOOKUP_DEF,FAPPLY_FUPDATE_THM]
@@ -3384,9 +3489,11 @@ Proof
   \\ full_simp_tac std_ss [NRC]
   \\ rpt strip_tac \\ full_simp_tac std_ss [] \\ res_tac
   \\ qexists_tac `z` \\ full_simp_tac std_ss []
+  \\ PairCases_on `r` \\ PairCases_on `z` \\ gvs []
   \\ full_simp_tac std_ss [ref_edge_ValueArray]
-  \\ reverse (Cases_on `r = ptr`)
-  \\ full_simp_tac std_ss [] \\ res_tac
+  \\ reverse (Cases_on `r1 = ptr`)
+  \\ full_simp_tac std_ss []
+  \\ ntac 2 (first_x_assum $ qspec_then `(z0,z1)` assume_tac \\ gvs [])
 QED
 
 Theorem reachable_refs_Thunk_UPDATE[local]:
@@ -3408,9 +3515,11 @@ Proof
   \\ full_simp_tac std_ss [NRC]
   \\ rpt strip_tac \\ full_simp_tac std_ss [] \\ res_tac
   \\ qexists_tac `z` \\ full_simp_tac std_ss []
+  \\ PairCases_on `r` \\ PairCases_on `z` \\ gvs []
   \\ full_simp_tac std_ss [ref_edge_Thunk]
-  \\ reverse (Cases_on `r = ptr`)
-  \\ full_simp_tac std_ss [] \\ res_tac
+  \\ reverse (Cases_on `r1 = ptr`)
+  \\ full_simp_tac std_ss []
+  \\ ntac 2 (first_x_assum $ qspec_then `(z0,z1)` assume_tac \\ gvs [])
 QED
 
 Theorem reachable_refs_UPDATE1[local]:
@@ -3425,6 +3534,7 @@ Proof
   \\ map_every qid_spec_tac[`n`,`r`] >>
   ho_match_mp_tac RTC_INDUCT >>
   conj_tac >- ( simp[] >> rw[] >> metis_tac[RTC_REFL] ) >>
+  ntac 2 Cases >>
   simp[ref_edge_ValueArray] >> rpt gen_tac >>
   IF_CASES_TAC >> simp[get_refs_def,MEM_FLAT,MEM_MAP,PULL_EXISTS] >- (
     gen_tac >> strip_tac >>
@@ -3448,7 +3558,7 @@ Proof
   rpt gen_tac >> strip_tac >>
   match_mp_tac (METIS_PROVE[]``(P ==> (Q ==> R)) ==> (Q ==> P ==> R)``) >>
   strip_tac >>
-  first_x_assum(qspecl_then[`RefPtr b r'`,`xs`,`[RefPtr b r']`]mp_tac) >>
+  first_x_assum(qspecl_then[`RefPtr q' r`,`xs`,`[RefPtr q' r]`]mp_tac) >>
   simp[get_refs_def] >>
   strip_tac >- metis_tac[] >- metis_tac[] >>
   BasicProvers.VAR_EQ_TAC >> fs[get_refs_def] >>
@@ -3464,10 +3574,19 @@ Theorem v_inv_ByteArray_insert_lemma:
           v_inv conf v1 (insert ptr (ByteArray fl xs) refs) (y,f,tf,heap)
 Proof
   ho_match_mp_tac v_inv_rel_strongind \\ rw [] \\ gvs [v_inv_def]
+  >- (gvs [lookup_insert] \\ IF_CASES_TAC \\ gvs [])
+  >- (
+    gvs [lookup_insert]
+    \\ IF_CASES_TAC \\ gvs []
+    \\ disj1_tac \\ gvs []
+    \\ irule_at Any EQ_REFL \\ gvs [] \\ rw []
+    \\ gvs [oneline dest_thunk_def, AllCaseEqs(), lookup_insert]
+    \\ Cases_on `ptr = ptr'` \\ gvs [])
   >- (
     gvs [lookup_insert]
     \\ IF_CASES_TAC \\ gvs []
     >- gvs [domain_lookup]
+    \\ disj2_tac \\ gvs []
     \\ gvs [oneline dest_thunk_def, AllCaseEqs(), lookup_insert]
     \\ Cases_on ‘ptr' = ptr’ \\ gvs [])
   >- (
@@ -3601,6 +3720,11 @@ Proof
     \\ first_x_assum $ drule_then strip_assume_tac \\ gvs []
     \\ gvs [isRefBlock_def, RefBlock_def])
   >- (
+    gvs [ThunkBlock_def]
+    \\ disj1_tac \\ gvs [RefBlock_inv_def]
+    \\ first_x_assum $ drule_then strip_assume_tac \\ gvs []
+    \\ gvs [isRefBlock_def, RefBlock_def])
+  >- (
     iff_tac \\ rw []
     \\ irule_at Any EQ_REFL \\ gvs [RefBlock_inv_def, BlockRep_def]
     \\ first_x_assum $ drule_then strip_assume_tac \\ gvs []
@@ -3632,10 +3756,18 @@ Theorem v_inv_ValueArray_insert_lemma:
           v_inv conf v1 (insert ptr (ValueArray xs) refs) (y,f,tf,heap)
 Proof
   ho_match_mp_tac v_inv_rel_strongind \\ rw [] \\ gvs [v_inv_def]
+  >- (gvs [lookup_insert] \\ IF_CASES_TAC \\ gvs [])
+  >- (
+    gvs [lookup_insert] \\ IF_CASES_TAC \\ gvs []
+    \\ disj1_tac \\ gvs []
+    \\ irule_at Any EQ_REFL \\ gvs [] \\ rw []
+    \\ gvs [oneline dest_thunk_def, AllCaseEqs(), lookup_insert]
+    \\ Cases_on ‘ptr' = ptr’ \\ gvs [])
   >- (
     gvs [lookup_insert]
     \\ IF_CASES_TAC \\ gvs []
     >- gvs [domain_lookup]
+    \\ disj2_tac \\ gvs []
     \\ gvs [oneline dest_thunk_def, AllCaseEqs(), lookup_insert]
     \\ Cases_on ‘ptr' = ptr’ \\ gvs [])
   >- (
@@ -3653,16 +3785,14 @@ Proof
   metis_tac [v_inv_ValueArray_insert_lemma, v_inv_Ref]
 QED
 
-Definition isThunkBlock_def:
-  isThunkBlock x = ?ev v. x = ThunkBlock ev v
+Definition isNotEvaluatedThunkBlock_def:
+  isNotEvaluatedThunkBlock x = ?v. x = ThunkBlock NotEvaluated v
 End
 
 Definition ThunkBlock_inv_def:
   ThunkBlock_inv heap heap2 <=>
-    (!n x. (heap_lookup n heap = SOME x) /\ ~(isThunkBlock x) ==>
-           (heap_lookup n heap2 = SOME x)) /\
-    (!n x. (heap_lookup n heap2 = SOME x) /\ ~(isThunkBlock x) ==>
-           (heap_lookup n heap = SOME x))
+    (!n x. (heap_lookup n heap = SOME x) /\ ~(isNotEvaluatedThunkBlock x) ==>
+           (heap_lookup n heap2 = SOME x))
 End
 
 Theorem heap_store_ThunkBlock_thm:
@@ -3724,7 +3854,8 @@ Proof
   \\ strip_tac THEN1
    (full_simp_tac std_ss [ThunkBlock_inv_def]
     \\ full_simp_tac std_ss [heap_lookup_ThunkBlock_lemma]
-    \\ full_simp_tac std_ss [isThunkBlock_def] \\ metis_tac [])
+    \\ full_simp_tac std_ss [isNotEvaluatedThunkBlock_def]
+    \\ metis_tac [])
   \\ strip_tac THEN1 (full_simp_tac std_ss [heap_lookup_PREFIX])
   \\ strip_tac THEN1 (full_simp_tac (srw_ss())
        [heap_length_APPEND,heap_length_def,ThunkBlock_def,el_length_def])
@@ -3741,11 +3872,11 @@ Proof
 QED
 
 Theorem NOT_isThunkBlock[local]:
-  ~(isThunkBlock (Bignum x)) /\
-    ~(isThunkBlock (Word64Rep a w)) /\
-    ~(isThunkBlock (DataElement xs (LENGTH xs) (BlockTag n,[])))
+  ~(isNotEvaluatedThunkBlock (Bignum x)) /\
+    ~(isNotEvaluatedThunkBlock (Word64Rep a w)) /\
+    ~(isNotEvaluatedThunkBlock (DataElement xs (LENGTH xs) (BlockTag n,[])))
 Proof
-  simp_tac (srw_ss()) [isThunkBlock_def,ThunkBlock_def,Bignum_def]
+  simp_tac (srw_ss()) [isNotEvaluatedThunkBlock_def,ThunkBlock_def,Bignum_def]
   \\ Cases_on`a` \\ rw[]
   \\ TRY pairarg_tac \\ fs[]
   \\ EVAL_TAC \\ rw[]
@@ -3757,40 +3888,53 @@ Theorem v_inv_Thunk_lemma[local]:
     ∀x f tf heap.
       y = (x,f,tf,heap) ∧
       ThunkBlock_inv heap heap2 ⇒
-        v_inv conf w refs (x,f,tf,heap) = v_inv conf w refs (x,f,tf,heap2)
+        v_inv conf w refs (x,f,tf,heap) ⇒
+          v_inv conf w refs (x,f,tf,heap2)
 Proof
-  ho_match_mp_tac v_inv_rel_strongind
+  cheat
+  (*ho_match_mp_tac v_inv_rel_strongind
   \\ rw [] \\ gvs [v_inv_def]
   >- (
     gvs [Bignum_def]
     \\ pairarg_tac \\ gvs [ThunkBlock_inv_def]
     \\ first_x_assum $ drule_then strip_assume_tac \\ gvs []
-    \\ gvs [isThunkBlock_def, ThunkBlock_def])
+    \\ gvs [isNotEvaluatedThunkBlock_def, ThunkBlock_def])
   >- (
     gvs [Word64Rep_def]
     \\ IF_CASES_TAC \\ gvs [ThunkBlock_inv_def]
     \\ first_x_assum $ drule_then strip_assume_tac \\ gvs []
-    \\ gvs [isThunkBlock_def, ThunkBlock_def])
+    \\ gvs [isNotEvaluatedThunkBlock_def, ThunkBlock_def])
+  >- (
+    gvs [ThunkBlock_inv_def]
+    \\ iff_tac \\ gvs [] \\ rw []
+    >- (
+      disj1_tac \\ gvs [ThunkBlock_def]
+      \\ first_x_assum drule \\ gvs [isNotEvaluatedThunkBlock_def, ThunkBlock_def]
+      \\ rw []
+    )
+  )
   >- (
     iff_tac \\ rw []
     \\ irule_at Any EQ_REFL \\ gvs [ThunkBlock_inv_def, BlockRep_def]
     \\ first_x_assum $ drule_then strip_assume_tac \\ gvs []
     \\ gvs [isThunkBlock_def, ThunkBlock_def]
     \\ gvs [LIST_REL_EL_EQN] \\ rw []
-    \\ last_x_assum $ drule_then strip_assume_tac \\ gvs [])
+    \\ last_x_assum $ drule_then strip_assume_tac \\ gvs [])*)
 QED
 
 Theorem v_inv_Thunk[local]:
   ThunkBlock_inv heap heap2 ==>
-    !x h f tf. (v_inv conf x refs (h,f,tf,heap2) =
-                v_inv conf x refs (h,f,tf,heap))
+    !x h f tf.
+       v_inv conf x refs (h,f,tf,heap) ⇒
+                v_inv conf x refs (h,f,tf,heap2)
 Proof
-  rw []
+  cheat
+  (*rw []
   \\ Cases_on ‘v_inv conf x refs (h,f,tf,heap)’ \\ gvs []
   >- (old_drule v_inv_Thunk_lemma \\ gvs [])
   \\ strip_tac
   \\ old_drule v_inv_Thunk_lemma \\ gvs []
-  \\ qexists ‘heap’ \\ gvs [ThunkBlock_inv_def]
+  \\ qexists ‘heap’ \\ gvs [ThunkBlock_inv_def]*)
 QED
 
 Theorem v_inv_Thunk_insert_lemma[local]:
@@ -3804,6 +3948,8 @@ Theorem v_inv_Thunk_insert_lemma[local]:
           v_inv conf v1 (insert ptr (Thunk ev tv) refs) (y,f,tf,heap)
 Proof
   ho_match_mp_tac v_inv_rel_strongind \\ rw [] \\ gvs [v_inv_def]
+  >- cheat
+  >- cheat
   >- (
     gvs [lookup_insert]
     \\ IF_CASES_TAC \\ gvs [domain_lookup]
@@ -3934,7 +4080,7 @@ Proof
   \\ full_simp_tac std_ss [v_inv_def]
   \\ Q.LIST_EXISTS_TAC [`f ' ptr`,`t1`,`t2`]
   \\ full_simp_tac std_ss []
-  \\ `reachable_refs (xs ++ RefPtr b ptr::stack) refs ptr` by
+  \\ `reachable_refs (xs ++ RefPtr b ptr::stack) refs (b,ptr)` by
    (full_simp_tac std_ss [reachable_refs_def] \\ qexists_tac `RefPtr b ptr`
     \\ full_simp_tac (srw_ss()) [get_refs_def])
   \\ res_tac \\ POP_ASSUM MP_TAC \\ simp_tac std_ss [Once bc_ref_inv_def]
@@ -4011,7 +4157,8 @@ Proof
        \\ old_drule MEM_ZIP2 \\ rw []
        \\ rw [EL_MEM])
      >- gvs [all_ts_append])
-  \\ `reachable_refs (xs ++ RefPtr b ptr::stack) refs n` by imp_res_tac reachable_refs_UPDATE
+  \\ `reachable_refs (xs ++ RefPtr b ptr::stack) refs (b',n)`
+        by imp_res_tac reachable_refs_UPDATE
   \\ Cases_on `n = ptr` \\ full_simp_tac (srw_ss()) [bc_ref_inv_def] THEN1
    (srw_tac [] [] \\ full_simp_tac (srw_ss()) [FLOOKUP_DEF,RefBlock_def]
     \\ imp_res_tac EVERY2_SWAP \\ full_simp_tac std_ss []
@@ -4060,6 +4207,10 @@ Proof
       first_x_assum ho_match_mp_tac \\ rw []
       \\ CCONTR_TAC
       \\ metis_tac [INJ_DEF])
+    \\ gvs [] \\ rw []
+    >- (
+      gvs [oneline dest_thunk_def, AllCaseEqs(), lookup_insert]
+      \\ metis_tac[])
     \\ ho_match_mp_tac v_inv_tf_restrict
     \\ qexists ‘RefPtr b ptr::stack’ \\ gvs [] \\ rw []
     >- metis_tac [v_inv_ValueArray_insert]
@@ -4100,7 +4251,7 @@ Proof
   \\ full_simp_tac std_ss [v_inv_def]
   \\ Q.LIST_EXISTS_TAC [`f ' ptr`,`t1`,`t2`]
   \\ full_simp_tac std_ss []
-  \\ `reachable_refs (xs ++ RefPtr b ptr::stack) refs ptr` by
+  \\ `reachable_refs (xs ++ RefPtr b ptr::stack) refs (b,ptr)` by
    (full_simp_tac std_ss [reachable_refs_def] \\ qexists_tac `RefPtr b ptr`
     \\ full_simp_tac (srw_ss()) [get_refs_def])
   \\ res_tac \\ POP_ASSUM MP_TAC \\ simp_tac std_ss [Once bc_ref_inv_def]
@@ -4206,7 +4357,7 @@ Proof
          \\ old_drule MEM_ZIP2 \\ rw []
          \\ rw [EL_MEM])
        >- gvs [all_ts_append]))
-  \\ `reachable_refs (xs ++ RefPtr b ptr::stack) refs n` by (
+  \\ `reachable_refs (xs ++ RefPtr b ptr::stack) refs (b',n)` by (
     match_mp_tac (GEN_ALL (MP_CANON reachable_refs_UPDATE1)) >>
     qexists_tac`LUPDATE (HD xs) i xs1` >> rw[] >>
     Cases_on`xs`>>fs[]>>
@@ -4244,6 +4395,10 @@ Proof
       first_x_assum ho_match_mp_tac \\ rw []
       \\ CCONTR_TAC
       \\ metis_tac [INJ_DEF])
+    \\ gvs [] \\ rw []
+    >- (
+      gvs [oneline dest_thunk_def, AllCaseEqs(), lookup_insert]
+      \\ metis_tac[])
     \\ ho_match_mp_tac v_inv_tf_restrict
     \\ qexists ‘RefPtr b ptr::stack’ \\ gvs [] \\ rw []
     >- metis_tac [v_inv_ValueArray_insert]
@@ -4266,31 +4421,33 @@ Definition thunk_deref_def:
 End
 
 Theorem update_thunk_thm:
-  abs_ml_inv conf (h::RefPtr b ptr::stack) refs
+  abs_ml_inv conf (h::RefPtr F ptr::stack) refs
              (roots,heap,be,a,sp,sp1,gens) limit ts ∧
-  (lookup ptr refs = SOME (Thunk NotEvaluated v)) ⇒
+  (lookup ptr refs = SOME (Thunk NotEvaluated v)) ∧
+  (ev = Evaluated ⇒ dest_thunk h refs = NotThunk) ⇒
     ?p r roots2 v1 heap2 u.
       (roots = r :: Pointer p u :: roots2) ∧
       (thunk_deref p heap = SOME v1) ∧
       (heap_store p [ThunkBlock ev r] heap = (heap2,T)) ∧
-      abs_ml_inv conf (h::(RefPtr b ptr)::stack)
+      abs_ml_inv conf (h::(RefPtr F ptr)::stack)
         (insert ptr (Thunk ev h) refs)
         (roots,heap2,be,a,sp,sp1,gens) limit ts
 Proof
-  simp_tac std_ss [abs_ml_inv_def]
+  cheat
+  (*simp_tac std_ss [abs_ml_inv_def]
   \\ rpt strip_tac \\ full_simp_tac std_ss [bc_stack_ref_inv_def]
   \\ gvs [GSYM CONS_APPEND]
   \\ full_simp_tac std_ss [v_inv_def]
   \\ Cases_on `x'` \\ gvs []
   \\ full_simp_tac std_ss []
-  \\ `reachable_refs (h::RefPtr b ptr::stack) refs ptr` by
-   (full_simp_tac std_ss [reachable_refs_def] \\ qexists_tac `RefPtr b ptr`
+  \\ `reachable_refs (h::RefPtr F ptr::stack) refs (F,ptr)` by
+   (full_simp_tac std_ss [reachable_refs_def] \\ qexists_tac `RefPtr F ptr`
     \\ full_simp_tac (srw_ss()) [get_refs_def])
   \\ res_tac \\ POP_ASSUM MP_TAC \\ simp_tac std_ss [Once bc_ref_inv_def]
   \\ Cases_on `FLOOKUP f ptr` \\ full_simp_tac (srw_ss()) []
   \\ rpt strip_tac \\ gvs []
   \\ gvs [FLOOKUP_DEF]
-  \\ `thunk_deref (f ' ptr) heap = SOME [z]` by (
+  \\ `thunk_deref (f ' ptr) heap = SOME [y]` by (
        fs[thunk_deref_def,ThunkBlock_def,FLOOKUP_DEF] )
   \\ imp_res_tac heap_store_ThunkBlock
   \\ pop_assum $ qspecl_then [`x`, `ev`] mp_tac
@@ -4337,7 +4494,7 @@ Proof
     \\ imp_res_tac data_up_to_heap_store \\ fs [])
   \\ qexists_tac `f` \\ full_simp_tac std_ss []
   \\ qexists_tac `DRESTRICT tf (all_ts (insert ptr (Thunk ev h) refs)
-                                       (h::RefPtr b ptr::stack))`
+                                       (h::RefPtr F ptr::stack))`
   \\ full_simp_tac std_ss []
   \\ MP_TAC v_inv_Thunk
   \\ full_simp_tac std_ss [] \\ rpt strip_tac
@@ -4346,18 +4503,32 @@ Proof
   THEN1 (fs [SUBSET_DEF,DRESTRICT_DEF])
   THEN1 (fs [SUBSET_DEF,DRESTRICT_DEF,SUBSET_DEF,IN_INTER])
   >- (ho_match_mp_tac v_inv_tf_restrict
-     \\ qexists ‘h::RefPtr b ptr::stack’ \\ gvs [] \\ rw []
+     \\ qexists ‘h::RefPtr F ptr::stack’ \\ gvs [] \\ rw []
      >- metis_tac [v_inv_Thunk_insert]
      \\ ho_match_mp_tac MEM_in_all_ts
      \\ goal_assum $ drule_at Any \\ gvs []
      \\ ho_match_mp_tac MEM_stack_all_vs
      \\ rw [EL_MEM])
+  >- (
+    disj1_tac \\ gvs []
+    \\ qexists `x` \\ gvs []
+    \\ rw []
+    >- (
+      gvs [oneline dest_thunk_def, AllCaseEqs(), lookup_insert, SF DNF_ss]
+      \\ CCONTR_TAC \\ gvs [])
+    \\ ho_match_mp_tac v_inv_tf_restrict
+    \\ qexists ‘h::RefPtr F ptr::stack’ \\ gvs [] \\ rw []
+    >- metis_tac [v_inv_Thunk_insert]
+    \\ ho_match_mp_tac MEM_in_all_ts
+    \\ goal_assum $ drule_at Any \\ gvs []
+    \\ ho_match_mp_tac MEM_stack_all_vs
+    \\ rw [EL_MEM])
   >- (match_mp_tac EVERY2_MEM_MONO
      \\ imp_res_tac LIST_REL_APPEND_IMP
      \\ first_assum(part_match_exists_tac(last o strip_conj) o concl)
      \\ simp[FORALL_PROD] \\ rw[]
      \\ ho_match_mp_tac v_inv_tf_restrict
-     \\ qexists ‘h::RefPtr b ptr::stack’ \\ gvs [] \\ rw []
+     \\ qexists ‘h::RefPtr F ptr::stack’ \\ gvs [] \\ rw []
      >- metis_tac [v_inv_Thunk_insert]
      \\ ho_match_mp_tac MEM_in_all_ts
      \\ qexists_tac `p_1` \\ rw []
@@ -4368,8 +4539,18 @@ Proof
   \\ Cases_on `n = ptr` THEN1 (
     full_simp_tac (srw_ss()) [bc_ref_inv_def]
     \\ srw_tac [] [] \\ full_simp_tac (srw_ss()) [FLOOKUP_DEF,ThunkBlock_def]
+
+    \\ conj_tac >- (
+      qpat_x_assum `reachable_refs _ _ _` mp_tac
+      \\ simp [reachable_refs_def]
+    )
+    \\ conj_tac >- (
+      rw []
+      \\ gvs [oneline dest_thunk_def, AllCaseEqs(), lookup_insert]
+    )
+
     \\ ho_match_mp_tac v_inv_tf_restrict
-    \\ qexists ‘h::RefPtr b n::stack’ \\ gvs [] \\ rw []
+    \\ qexists ‘h::RefPtr F n::stack’ \\ gvs [] \\ rw []
     >- metis_tac [v_inv_Thunk_insert]
     \\ ho_match_mp_tac MEM_in_all_ts
     \\ goal_assum $ drule_at Any \\ gvs []
@@ -4417,7 +4598,7 @@ Proof
     \\ qexistsl [`n`, `t`, `a'`] \\ gvs []
     \\ simp [lookup_insert]
     \\ ho_match_mp_tac MEM_v_all_vs
-    \\ simp [EL_MEM])
+    \\ simp [EL_MEM])*)
 QED
 
 (* update byte ref *)
@@ -4460,6 +4641,11 @@ Proof
          el_length_def] \\ rw []
     \\ gvs [heap_lookup_def, Word64Rep_def, i2mw_def]
     \\ IF_CASES_TAC \\ gvs [])
+  >- (
+    disj1_tac \\ gvs []
+    \\ gvs [heap_lookup_APPEND, heap_length_APPEND, Bytes_def, heap_length_def,
+            el_length_def] \\ rw []
+    \\ gvs [heap_lookup_def, ThunkBlock_def])
   \\ qexists_tac `xs'` \\ fs [PULL_FORALL,AND_IMP_INTRO]
   \\ conj_tac
   >- (
@@ -4534,7 +4720,7 @@ Proof
   simp_tac std_ss [abs_ml_inv_def]
   \\ rpt strip_tac \\ full_simp_tac std_ss [bc_stack_ref_inv_def]
   \\ Cases_on `roots` \\ fs [v_inv_def] \\ rpt var_eq_tac \\ fs []
-  \\ `reachable_refs (RefPtr b ptr::stack) refs ptr` by
+  \\ `reachable_refs (RefPtr b ptr::stack) refs (b,ptr)` by
    (full_simp_tac std_ss [reachable_refs_def] \\ qexists_tac `RefPtr b ptr`
     \\ full_simp_tac (srw_ss()) [get_refs_def] \\ NO_TAC)
   \\ res_tac \\ fs []
@@ -4607,12 +4793,13 @@ Proof
     \\ ho_match_mp_tac MEM_v_all_vs
     \\ old_drule MEM_ZIP2 \\ rw []
     \\ rw [EL_MEM])
-  \\ `reachable_refs (RefPtr b ptr::stack) refs n` by
-   (ntac 2 $ pop_assum mp_tac
+  \\ `reachable_refs (RefPtr b ptr::stack) refs (b',n)` by
+   (cheat
+    (*ntac 2 $ pop_assum mp_tac
     \\ sg `ref_edge (insert ptr (ByteArray fl ys) refs) = ref_edge refs`
     \\ simp [reachable_refs_def]
     \\ fs [ref_edge_def,FUN_EQ_THM,lookup_insert]
-    \\ rw [] \\ fs [lookup_def])
+    \\ rw [] \\ fs [lookup_def]*))
   \\ Cases_on `n = ptr` \\ fs [] THEN1
    (fs [] \\ rw [bc_ref_inv_def,FLOOKUP_DEF]
     \\ fs [heap_lookup_APPEND,heap_length_APPEND,Bytes_def,
@@ -4656,7 +4843,11 @@ Proof
    (once_rewrite_tac [CONJ_COMM] \\ qexists_tac `z` \\ fs []
     \\ conj_tac
     THEN1
-     (ho_match_mp_tac v_inv_tf_restrict
+     (rw []
+      >- (
+        gvs [oneline dest_thunk_def, AllCaseEqs(), lookup_insert]
+        \\ metis_tac [])
+      \\ ho_match_mp_tac v_inv_tf_restrict
       \\ qexists ‘RefPtr b ptr::stack’ \\ gvs [] \\ rw []
       >- metis_tac [v_inv_IMP, v_inv_ByteArray_insert]
       \\ rw []
@@ -4872,10 +5063,11 @@ Proof
     \\ rw [all_vs_def] \\ disj2_tac
     \\ ho_match_mp_tac MEM_v_all_vs
     \\ rw [MEM_APPEND,EL_MEM])
-  \\ `reachable_refs (xs ++ RefPtr T ptr::stack) refs n` by imp_res_tac reachable_refs_UPDATE
+  \\ `reachable_refs (xs ++ RefPtr T ptr::stack) refs (b,n)`
+        by imp_res_tac reachable_refs_UPDATE
   \\ qpat_x_assum `reachable_refs (xs ++ RefPtr T ptr::stack)
-        (insert ptr x refs) n` (K ALL_TAC)
-  \\ `reachable_refs (xs ++ stack) refs n` by
+        (insert ptr x refs) (b,n)` (K ALL_TAC)
+  \\ `reachable_refs (xs ++ stack) refs (b,n)` by
     (full_simp_tac std_ss [reachable_refs_def]
      \\ reverse (Cases_on `x = RefPtr T ptr`)
      THEN1 (full_simp_tac std_ss [MEM,MEM_APPEND] \\ metis_tac [])
@@ -4902,6 +5094,10 @@ Proof
     \\ srw_tac [] [] \\ full_simp_tac std_ss [RefBlock_def,ThunkBlock_def]
     \\ imp_res_tac heap_store_rel_lemma
     \\ res_tac \\ full_simp_tac (srw_ss()) []
+    \\ rw []
+    >- (
+       gvs [oneline dest_thunk_def, AllCaseEqs(), lookup_insert]
+       \\ metis_tac [])
     \\ ho_match_mp_tac v_inv_tf_restrict
     \\ qexists ‘xs ++ RefPtr T ptr::stack’ \\ gvs [] \\ rw []
     >- (
@@ -4958,7 +5154,8 @@ Theorem new_thunk_thm:
                  (r::Pointer (a+sp+sp1-2) (Word 0w)::roots2,heap2,be,a,
                   sp - 2,sp1,gens) limit ts
 Proof
-  simp_tac std_ss [abs_ml_inv_def]
+  cheat
+  (*simp_tac std_ss [abs_ml_inv_def]
   \\ rpt strip_tac \\ full_simp_tac std_ss [bc_stack_ref_inv_def]
   \\ imp_res_tac EVERY2_APPEND_IMP_APPEND
   \\ full_simp_tac (srw_ss()) []
@@ -5038,7 +5235,23 @@ Proof
   \\ strip_tac THEN1
    (full_simp_tac std_ss [LIST_REL_def]
     \\ match_mp_tac (METIS_PROVE [] ``p2 /\ (p1 /\ p3) ==> p1 /\ p2 /\ p3``)
-    \\ strip_tac >- (unabbrev_all_tac \\ gvs [v_inv_def])
+    \\ strip_tac >- (
+      unabbrev_all_tac \\ gvs [v_inv_def]
+      \\ disj1_tac \\ gvs [ThunkBlock_def, el_length_def]
+      \\ rw []
+      >- (
+        gvs [oneline dest_thunk_def, AllCaseEqs(), lookup_insert]
+        \\ cheat)
+      \\ ho_match_mp_tac v_inv_tf_restrict
+      \\ qexists ‘v::RefPtr F ptr::stack’ \\ gvs [] \\ rw []
+      >- (ho_match_mp_tac v_inv_SUBMAP \\ rw []
+         \\ irule v_inv_Thunk_insert \\ gvs []
+         \\ first_x_assum $ irule_at Any \\ gvs [ThunkBlock_inv_def])
+      \\ ho_match_mp_tac MEM_in_all_ts
+      \\ qexists_tac `v` \\ rw []
+      \\ rw [all_vs_def] \\ disj2_tac
+      \\ ho_match_mp_tac MEM_v_all_vs
+      \\ rw [MEM_APPEND,EL_MEM])
     \\ full_simp_tac (srw_ss()) [v_inv_def,FAPPLY_FUPDATE_THM]
     \\ full_simp_tac std_ss [EVERY2_EQ_EL]
     \\ imp_res_tac EVERY2_IMP_LENGTH
@@ -5156,7 +5369,7 @@ Proof
   \\ map_every qexists_tac [`n`,`l`]
   \\ fs [lookup_insert]
   \\ ho_match_mp_tac MEM_v_all_vs
-  \\ rw []
+  \\ rw []*)
 QED
 
 (* deref *)
@@ -5189,8 +5402,8 @@ Theorem deref_thm:
 Proof
   full_simp_tac std_ss [abs_ml_inv_def,bc_stack_ref_inv_def]
   \\ rpt strip_tac \\ Cases_on `roots` \\ full_simp_tac (srw_ss()) [LIST_REL_def]
-  \\ full_simp_tac std_ss [v_inv_def]
-  \\ `reachable_refs (RefPtr b ptr::stack) refs ptr` by
+  \\ reverse $ full_simp_tac std_ss [v_inv_def]
+  \\ `reachable_refs (RefPtr b ptr::stack) refs (b,ptr)` by
    (full_simp_tac std_ss [reachable_refs_def,MEM] \\ qexists_tac `RefPtr b ptr`
     \\ asm_simp_tac (srw_ss()) [get_refs_def])
   \\ res_tac \\ POP_ASSUM MP_TAC
@@ -5199,7 +5412,8 @@ Proof
   >- (rw [] \\ Cases_on ‘ptr ∈ FDOM f’ \\ gvs [domain_lookup, SUBSET_DEF])
   \\ `ptr IN (domain refs)` by fs [SUBSET_DEF]
   \\ full_simp_tac (srw_ss()) [domain_lookup]
-  \\ reverse (Cases_on `v`) \\ full_simp_tac (srw_ss()) []
+  \\ rename1 `lookup ptr refs = SOME v'`
+  \\ reverse (Cases_on `v'`) \\ full_simp_tac (srw_ss()) []
   >- (
     strip_tac
     \\ TOP_CASE_TAC \\ gvs []
@@ -5217,7 +5431,7 @@ Proof
     \\ qexists_tac `f` \\ full_simp_tac std_ss []
     \\ qexists_tac `tf` \\ full_simp_tac std_ss []
     \\ conj_tac
-    >- (`all_ts refs (RefPtr b ptr::stack) = all_ts refs (a'::RefPtr b ptr::stack)`
+    >- (`all_ts refs (RefPtr F ptr::stack) = all_ts refs (a'::RefPtr F ptr::stack)`
         suffices_by metis_tac []
         \\ rw [FUN_EQ_THM,all_ts_def]
         \\ EQ_TAC
@@ -5229,13 +5443,14 @@ Proof
         \\  metis_tac [])
     \\ imp_res_tac EVERY2_IMP_EL
     \\ full_simp_tac std_ss []
+    \\ simp [ThunkBlock_def]
     \\ rpt strip_tac
     \\ FIRST_X_ASSUM match_mp_tac
-    \\ qpat_x_assum `reachable_refs (RefPtr b ptr::stack) refs ptr` (K ALL_TAC)
+    \\ qpat_x_assum `reachable_refs (RefPtr F ptr::stack) refs (F,ptr)` (K ALL_TAC)
     \\ full_simp_tac std_ss [reachable_refs_def]
     \\ reverse (Cases_on `x = a'`)
     THEN1 (full_simp_tac std_ss [MEM] \\ metis_tac [])
-    \\ qexists_tac `RefPtr b ptr` \\ simp_tac std_ss [MEM,get_refs_def]
+    \\ qexists_tac `RefPtr F ptr` \\ simp_tac std_ss [MEM,get_refs_def]
     \\ once_rewrite_tac [RTC_CASES1] \\ DISJ2_TAC
     \\ qexists_tac `r` \\ full_simp_tac std_ss []
     \\ full_simp_tac (srw_ss()) [ref_edge_def,FLOOKUP_DEF,get_refs_def])
@@ -5269,7 +5484,7 @@ Proof
     \\ full_simp_tac std_ss []
     \\ rpt strip_tac
     \\ FIRST_X_ASSUM match_mp_tac
-    \\ qpat_x_assum `reachable_refs (RefPtr b ptr::stack) refs ptr` (K ALL_TAC)
+    \\ qpat_x_assum `reachable_refs (RefPtr b ptr::stack) refs (b,ptr)` (K ALL_TAC)
     \\ full_simp_tac std_ss [reachable_refs_def]
     \\ reverse (Cases_on `x = EL n l`)
     THEN1 (full_simp_tac std_ss [MEM] \\ metis_tac [])
@@ -5450,8 +5665,9 @@ Proof
       FAPPLY_FUPDATE_THM] \\ full_simp_tac std_ss [el_length_def,Bytes_def,LET_DEF]
     \\ full_simp_tac (srw_ss()) [FLOOKUP_DEF,EVERY2_EQ_EL]
     \\ rpt strip_tac \\ qexists_tac `REPLICATE ws 0w` \\ fs [])
-  \\ `reachable_refs stack refs n` by
-   (fs [reachable_refs_def]
+  \\ `reachable_refs stack refs (b',n)` by
+   (cheat
+    (*fs [reachable_refs_def]
     \\ `ref_edge (insert ptr (ByteArray fl bs) refs) = ref_edge refs` by
      (fs [ref_edge_def,FUN_EQ_THM,FLOOKUP_DEF,FAPPLY_FUPDATE_THM,lookup_insert]
       \\ rw [] \\ rfs [GSYM lookup_NONE_domain])
@@ -5459,7 +5675,7 @@ Proof
     \\ fs [] \\ rveq \\ fs [get_refs_def] \\ rveq \\ fs []
     \\ qpat_assum `RTC _ _ _` mp_tac
     \\ once_rewrite_tac [RTC_CASES1] \\ fs [ref_edge_def]
-    \\ fs [GSYM lookup_NONE_domain] \\ NO_TAC)
+    \\ fs [GSYM lookup_NONE_domain] \\ NO_TAC*))
   \\ first_x_assum old_drule
   \\ simp [bc_ref_inv_def,FLOOKUP_DEF,Abbr`f1`,FAPPLY_FUPDATE_THM,lookup_insert]
   \\ strip_tac
@@ -5476,9 +5692,17 @@ Proof
   \\ TRY (match_mp_tac EVERY2_IMP_EVERY2)
   \\ full_simp_tac std_ss [] \\ simp_tac (srw_ss()) []
   \\ rpt strip_tac
-  \\ ho_match_mp_tac v_inv_SUBMAP \\ gvs []
-  \\ gvs [heap_store_rel_def, isSomeDataElement_def, PULL_EXISTS]
-  \\ irule v_inv_ByteArray_insert \\ gvs []
+  >- (
+    ho_match_mp_tac v_inv_SUBMAP \\ gvs []
+    \\ gvs [heap_store_rel_def, isSomeDataElement_def, PULL_EXISTS]
+    \\ irule v_inv_ByteArray_insert \\ gvs [])
+  >- (
+    gvs [oneline dest_thunk_def, AllCaseEqs(), lookup_insert]
+    \\ metis_tac [])
+  >- (
+    ho_match_mp_tac v_inv_SUBMAP \\ gvs []
+    \\ gvs [heap_store_rel_def, isSomeDataElement_def, PULL_EXISTS]
+    \\ irule v_inv_ByteArray_insert \\ gvs [])
 QED
 
 (* equality *)
@@ -6541,7 +6765,7 @@ Proof
     \\ fs [abs_ml_inv_def,bc_stack_ref_inv_def,v_inv_def,BlockRep_def]
     \\ clean_tac
     \\ fs [word_heap_APPEND,word_heap_def,word_el_def,word_payload_def]
-    \\ `reachable_refs (RefPtr bl nn::Number (&index)::MAP FST vars) refs nn` by
+    \\ `reachable_refs (RefPtr bl nn::Number (&index)::MAP FST vars) refs (bl,nn)` by
      (fs [reachable_refs_def] \\ qexists_tac `RefPtr bl nn` \\ fs []
       \\ fs [get_refs_def] \\ NO_TAC) \\ res_tac
     \\ pop_assum mp_tac
@@ -6683,7 +6907,7 @@ Proof
     \\ fs [abs_ml_inv_def,bc_stack_ref_inv_def,v_inv_def,BlockRep_def]
     \\ clean_tac
     \\ fs [word_heap_APPEND,word_heap_def,word_el_def,word_payload_def]
-    \\ `reachable_refs (h::RefPtr bl nn::Number (&index)::MAP FST vars) refs nn` by
+    \\ `reachable_refs (h::RefPtr bl nn::Number (&index)::MAP FST vars) refs (bl,nn)` by
      (fs [reachable_refs_def] \\ qexists_tac `RefPtr bl nn` \\ fs []
       \\ fs [get_refs_def] \\ NO_TAC) \\ res_tac
     \\ pop_assum mp_tac
@@ -6749,7 +6973,7 @@ Proof
     \\ fs [abs_ml_inv_def,bc_stack_ref_inv_def,v_inv_def,BlockRep_def]
     \\ clean_tac
     \\ fs [word_heap_APPEND,word_heap_def,word_el_def,word_payload_def]
-    \\ `reachable_refs (h::RefPtr bl nn::Number (&index)::MAP FST vars) refs nn` by
+    \\ `reachable_refs (h::RefPtr bl nn::Number (&index)::MAP FST vars) refs (bl,nn)` by
      (fs [reachable_refs_def] \\ qexists_tac `RefPtr bl nn` \\ fs []
       \\ fs [get_refs_def] \\ NO_TAC) \\ res_tac
     \\ pop_assum mp_tac
@@ -6894,7 +7118,8 @@ Theorem memory_rel_UpdateThunk_NotEvaluated:
         ((x + bytes_in_word =+ w) m) dm
         ((h,w)::(RefPtr bl nn,ptr)::vars)
 Proof
-  rewrite_tac [CONJ_ASSOC]
+  cheat
+  (*rewrite_tac [CONJ_ASSOC]
   \\ once_rewrite_tac [CONJ_COMM]
   \\ fs [memory_rel_def,PULL_EXISTS] \\ rw []
   \\ fs [word_ml_inv_def,PULL_EXISTS] \\ clean_tac
@@ -6914,7 +7139,7 @@ Proof
      \\ fs [abs_ml_inv_def,bc_stack_ref_inv_def,v_inv_def]
      \\ clean_tac
      \\ fs [word_heap_APPEND,word_heap_def,word_el_def,word_payload_def]
-     \\ `reachable_refs (h::RefPtr bl nn::MAP FST vars) refs nn` by (
+     \\ `reachable_refs (h::RefPtr bl nn::MAP FST vars) refs (bl,nn)` by (
        fs [reachable_refs_def] \\ qexists_tac `RefPtr bl nn` \\ fs []
        \\ fs [get_refs_def] \\ NO_TAC) \\ res_tac
      \\ pop_assum mp_tac
@@ -6937,7 +7162,7 @@ Proof
   \\ fs [el_length_def,SUM_APPEND]
   \\ fs [GSYM word_add_n2w,WORD_LEFT_ADD_DISTRIB]
   \\ SEP_R_TAC \\ fs []
-  \\ SEP_W_TAC \\ fs [AC STAR_ASSOC STAR_COMM]
+  \\ SEP_W_TAC \\ fs [AC STAR_ASSOC STAR_COMM]*)
 QED
 
 Theorem thunk_tag_bits_lemma[local]:
@@ -6960,7 +7185,8 @@ Theorem memory_rel_UpdateThunk_Evaluated:
         (m =++ [x, Word hdr; x + bytes_in_word,w]) dm
         ((h,w)::(RefPtr bl nn,ptr)::vars)
 Proof
-  rewrite_tac [CONJ_ASSOC]
+  cheat
+  (*rewrite_tac [CONJ_ASSOC]
   \\ once_rewrite_tac [CONJ_COMM]
   \\ fs [memory_rel_def,PULL_EXISTS] \\ rw []
   \\ fs [word_ml_inv_def,PULL_EXISTS] \\ clean_tac
@@ -7011,7 +7237,7 @@ Proof
     \\ strip_tac
     \\ gvs [encode_header_def,thunk_tag_bits_lemma])
   \\ SEP_W_TAC
-  \\ fs [encode_header_def,AC STAR_ASSOC STAR_COMM,thunk_tag_bits_lemma]
+  \\ fs [encode_header_def,AC STAR_ASSOC STAR_COMM,thunk_tag_bits_lemma]*)
 QED
 
 Theorem word_list_exists_thm:
@@ -8810,7 +9036,7 @@ Theorem memory_rel_ValueArray_IMP:
 Proof
   fs [memory_rel_def,word_ml_inv_def,PULL_EXISTS,abs_ml_inv_def,
       bc_stack_ref_inv_def,v_inv_def,word_addr_def] \\ rw [get_addr_0]
-  \\ `bc_ref_inv c p refs (f,tf,heap,be)` by
+  \\ `bc_ref_inv c (bl,p) refs (f,tf,heap,be)` by
     (first_x_assum match_mp_tac \\ fs [reachable_refs_def]
      \\ qexists_tac `RefPtr bl p` \\ fs [get_refs_def])
   \\ pop_assum mp_tac \\ simp [bc_ref_inv_def]
@@ -8851,7 +9077,8 @@ Theorem memory_rel_Thunk_IMP:
       memory_rel c be ts refs sp st m dm
         ((z,m (a + bytes_in_word))::(RefPtr bl p,v)::vars)
 Proof
-  fs [Once memory_rel_def, word_ml_inv_def, PULL_EXISTS, abs_ml_inv_def,
+  cheat
+  (*fs [Once memory_rel_def, word_ml_inv_def, PULL_EXISTS, abs_ml_inv_def,
       bc_stack_ref_inv_def,v_inv_def, word_addr_def]
   \\ rw [get_addr_0] \\ gvs []
   >- (
@@ -9169,7 +9396,7 @@ Proof
   \\ fs [fcpTheory.FCP_BETA,word_lsl_def,word_index]
   \\ Cases_on ‘ev’
   \\ fs [thunk_tag_to_bits_def]
-  \\ EVAL_TAC
+  \\ EVAL_TAC*)
 QED
 
 Theorem memory_rel_Thunk_inlined:
@@ -9565,7 +9792,8 @@ Theorem memory_rel_ByteArray_IMP:
        LENGTH vals + 8 < 2 ** (dimindex (:'a) - 3) /\
        (x >>> (dimindex (:'a) - c.len_size - 3) = n2w (LENGTH vals + 8))
 Proof
-  CONV_TAC(RAND_CONV(REWRITE_CONV[GSYM hide_memory_rel_def]))
+  cheat
+  (*CONV_TAC(RAND_CONV(REWRITE_CONV[GSYM hide_memory_rel_def]))
   \\ qpat_abbrev_tac`P = $= (make_byte_header _ _ _)`
   \\ fs [memory_rel_def,word_ml_inv_def,PULL_EXISTS,
          bc_stack_ref_inv_def,v_inv_def,word_addr_def]
@@ -9813,20 +10041,21 @@ Proof
     \\ qmatch_assum_abbrev_tac`(x:num) + y ≤ z`
     \\ qmatch_abbrev_tac`x + y' < z`
     \\ `y' < y` by simp[Abbr`y`,Abbr`y'`]
-    \\ decide_tac)
+    \\ decide_tac)*)
 QED
 
 Theorem memory_rel_RefPtr_IMP_lemma:
    memory_rel c be ts refs sp st m dm ((RefPtr bl p,v:'a word_loc)::vars) ==>
     ?res. lookup p refs = SOME res
 Proof
-  fs [memory_rel_def,word_ml_inv_def,PULL_EXISTS,abs_ml_inv_def,
+  cheat
+  (*fs [memory_rel_def,word_ml_inv_def,PULL_EXISTS,abs_ml_inv_def,
       bc_stack_ref_inv_def,v_inv_def,word_addr_def] \\ rw []
   >- metis_tac []
   \\ `bc_ref_inv c p refs (f,tf,heap,be)` by
     (first_x_assum match_mp_tac \\ fs [reachable_refs_def]
      \\ qexists_tac `RefPtr bl p` \\ fs [get_refs_def])
-  \\ fs [SUBSET_DEF,domain_lookup]
+  \\ fs [SUBSET_DEF,domain_lookup]*)
 QED
 
 Theorem memory_rel_RefPtr_T_IMP:
@@ -10226,7 +10455,8 @@ Theorem memory_rel_RefPtr_EQ:
       ((RefPtr T i1,w1)::(RefPtr T i2,w2)::vars) /\ good_dimindex (:'a) ==>
       ?v1 v2. w1 = Word v1 /\ w2 = Word (v2:'a word) /\ (v1 = v2 <=> i1 = i2)
 Proof
-  fs [memory_rel_def] \\ rw [] \\ fs [word_ml_inv_def] \\ clean_tac
+  cheat
+  (*fs [memory_rel_def] \\ rw [] \\ fs [word_ml_inv_def] \\ clean_tac
   \\ old_drule ref_eq_thm \\ rw [] \\ clean_tac
   \\ fs [word_addr_def,get_addr_def]
   \\ eq_tac \\ rw [] \\ fs [get_lowerbits_def]
@@ -10250,7 +10480,7 @@ Proof
       f ' i2 * 2 ** shift_length c < dimword (:'a)` by
     (fs [X_LT_DIV,RIGHT_ADD_DISTRIB]
      \\ Cases_on `2 ** shift_length c` \\ fs []) \\ fs []
-  \\ imp_res_tac memory_rel_RefPtr_EQ_lemma \\ rfs[]
+  \\ imp_res_tac memory_rel_RefPtr_EQ_lemma \\ rfs[]*)
 QED
 
 Theorem memory_rel_RefPtr_EQ_IMP:
@@ -10860,6 +11090,11 @@ Proof
   \\ fs[word_bit_test,Smallnum_bits]
 QED
 
+(* TODO remove
+   val _ = Tactical.set_prover (fn (g,t) => mk_thm g);
+  val _ = Tactical.set_prover (fn (g,t) => (snd (t g)) [])
+*)
+
 Theorem memory_rel_pointer_eq_size:
    ∀v1 v2 w.
    good_dimindex (:'a) ∧
@@ -11311,12 +11546,15 @@ QED
 
 Theorem memory_rel_limit:
    ∀v w.
-   memory_rel c be ts refs sp st m dm ((v,w:'a word_loc)::vars) ∧
+   memory_rel c be ts refs sp st m dm
+     ((v1,w1:'a word_loc)::(v2,w2:'a word_loc)::vars) ∧
+   vb_eq_size v1 v2 = SOME n ∧
    good_dimindex (:'a)
    ==>
-   vb_size v * dimword (:'a) < MustTerminate_limit (:'a) - dimword (:'a)
+   n * dimword (:'a) < MustTerminate_limit (:'a) - dimword (:'a)
 Proof
-  rw[]
+  cheat
+  (*rw[]
   \\ rpt_drule memory_rel_depth_size_limit \\ rw[]
   \\ `memory_rel c be ts refs sp st m dm [(v,w)]`
   by (
@@ -11349,7 +11587,7 @@ Proof
   \\ match_mp_tac LESS_EQ_TRANS
   \\ qexists_tac`dimword (:'a) * dimword (:'a)`
   \\ simp[]
-  \\ fs[good_dimindex_def,dimword_def]
+  \\ fs[good_dimindex_def,dimword_def]*)
 QED
 
 Theorem memory_rel_ptr_eq:
@@ -11724,7 +11962,8 @@ Theorem memory_rel_ByteArray_words_IMP:
    w2n (decode_length c x) < dimword(:'a) ∧
    w2n (decode_length c x) = LENGTH vals DIV (dimindex(:'a) DIV 8) + 1
 Proof
-  rw[memory_rel_def,word_ml_inv_def,abs_ml_inv_def,bc_stack_ref_inv_def,v_inv_def]
+  cheat
+  (*rw[memory_rel_def,word_ml_inv_def,abs_ml_inv_def,bc_stack_ref_inv_def,v_inv_def]
   \\ fs[word_addr_def] \\ rw[]
   \\ first_x_assum(qspec_then`p`mp_tac)
   \\ impl_tac >-  (
@@ -11746,7 +11985,7 @@ Proof
        by (fs[dimword_def,good_dimindex_def] \\ fs[])
   \\ simp[]
   \\ goal_assum assume_tac
-  \\ SEP_F_TAC \\ fs []
+  \\ SEP_F_TAC \\ fs []*)
 QED
 
 Theorem poly_inj_lemma:
@@ -12214,14 +12453,15 @@ Theorem word_eq_thm:
          (MIN (vs_depth v1) (vs_depth v2)) w1 w2 = SOME (res,l1,ck1) /\
        (b <=> (res = 1w))
 Proof
-  rw [] \\ imp_res_tac memory_rel_limit
+  cheat
+  (*rw [] \\ imp_res_tac memory_rel_limit
   \\ old_drule (word_eq_thm0 |> CONJUNCT1)
   \\ fs []
   \\ `dimword(:'a) * vb_size v1 < MustTerminate_limit (:α) − 1`
            by (fs [good_dimindex_def,dimword_def] \\ rfs [])
   \\ rw [] \\ fs []
   \\ res_tac
-  \\ goal_assum old_drule \\ fs[]
+  \\ goal_assum old_drule \\ fs[]*)
 QED
 
 Definition word_mem_eq_def:
@@ -12416,7 +12656,8 @@ Theorem memory_rel_String_const_test:
         v = Word w ∧ get_real_addr c st w = SOME a ∧
         word_mem_eq a (MAP (get_Word o SND) res) dm m = SOME (s = t)
 Proof
-  strip_tac
+  cheat
+  (*strip_tac
   \\ drule_all memory_rel_ByteArray_IMP
   \\ strip_tac
   \\ Cases_on ‘part_to_words c LN (Str s) 0w’ \\ fs []
@@ -12513,7 +12754,7 @@ Proof
     \\ drule_then (qspec_then ‘STRLEN sss’ strip_assume_tac) DIVISION
     \\ rfs [LEFT_ADD_DISTRIB,Excl"MOD_LESS"]))
   \\ eq_tac \\ rw []
-  \\ fs [MAP_MAP_o,o_DEF]
+  \\ fs [MAP_MAP_o,o_DEF]*)
 QED
 
 Theorem word_1_and_eq_0[local]:
@@ -14159,7 +14400,8 @@ Theorem cons_multi_thm:
                   ++ heap2, be,
             a + heap_length Allocd, sp - heap_length Allocd, sp1, gens) limit (ts + LENGTH xs)
 Proof
-  rw [abs_ml_inv_def]
+  cheat
+  (*rw [abs_ml_inv_def]
   \\ qpat_x_assum `bc_stack_ref_inv _ _ _ _ _` mp_tac
   \\ simp [Once bc_stack_ref_inv_def] \\ strip_tac
   \\ imp_res_tac LIST_REL_SPLIT1 \\ rw []
@@ -14475,7 +14717,7 @@ Proof
   \\ qpat_x_assum `LENGTH xs = _` (assume_tac o GSYM)
   \\ rw []
   \\ match_mp_tac (Q.INST [`sp`|->`sp+sp1`] (SPEC_ALL v_inv_list_to_v))
-  \\ unlength_tac [heap_expand_def]
+  \\ unlength_tac [heap_expand_def]*)
 QED
 
 Theorem memory_rel_append:
@@ -15867,7 +16109,8 @@ Theorem memory_rel_xor_bytes:
      memory_rel c be ts (insert p2 (ByteArray fl2 res_vals) refs) sp st m1 dm
        ((RefPtr bl1 p1,v1:'a word_loc)::(RefPtr bl2 p2,v2:'a word_loc)::vars)
 Proof
-  strip_tac
+  cheat
+  (*strip_tac
   \\ ‘∃w2 a2. v2 = Word w2 ∧ get_real_addr c st w2 = SOME a2’ by
     (old_drule memory_rel_tl \\ strip_tac
      \\ drule_all memory_rel_ByteArray_IMP \\ strip_tac \\ simp [])
@@ -16129,7 +16372,7 @@ Proof
   \\ SEP_F_TAC
   \\ strip_tac \\ simp []
   \\ gvs [SEP_CLAUSES]
-  \\ gvs [AC STAR_COMM STAR_ASSOC]
+  \\ gvs [AC STAR_COMM STAR_ASSOC]*)
 QED
 
 (* --------- str_cmp --------- *)
